iris/WpUserExec.v
@@ -6017,6 +6017,268 @@ Section WpUserExec.
     iExact "Hfmap".
   Qed.
 
+  Lemma ustep_rtype2 (mk2 : mword 5 -> mword 5 -> mword 5 -> instruction) (f : mword 64 -> mword 64 -> mword 64)
+      (va : mword 64) (vpn : mword 27) (ie : uwalk_info) (w : mword 32)
+      (rs2 rs1 rd : mword 5)
+      (ms_v sc_v stval_v sepc_v : mword 64)
+      (g : gmap regidx (mword 64))
+      (tlbvec : vec (option TLB_Entry) (2 ^ 6))
+      E (Φ : mval -> iProp Σ) :
+    ↑minstretN ⊆ E ->
+    (* the op's register-generic execute fact (nonzero-rd form) *)
+    (forall (rs2' rs1' rd' : mword 5) s, uint rd' <> 0 ->
+       exec (execute (mk2 rs2' rs1' rd')) s
+       = Some (RETIRE_SUCCESS,
+               set_reg s (R_bitvector_64 (gpr_of_Z (uint rd')))
+                 (regval_into_reg
+                    (f (if Z.eqb (uint rs1') 0 then zero_reg
+                        else register_lookup
+                               (R_bitvector_64 (gpr_of_Z (uint rs1'))) s.(sregs))
+                       (if Z.eqb (uint rs2') 0 then zero_reg
+                        else register_lookup
+                               (R_bitvector_64 (gpr_of_Z (uint rs2'))) s.(sregs)))))) ->
+    is_lpad_instruction (mk2 rs2 rs1 rd) = false ->
+    upt_tlb_ok spec tlbvec ->
+    (* fetch-hit facts *)
+    vec_access_dec tlbvec (tlb_hash (__id 39) vpn) = Some (upt_entry vpn ie) ->
+    uw_check_ok (InstructionFetch tt) ie ->
+    update_PTE_Bits (uw_pte0 ie) (InstructionFetch tt) = None ->
+    _get_PTE_Ext_PBMT (ext_bits_of_PTE (uw_pte0 ie)) = ('b"00" : mword 2) ->
+    (forall j : nat, (j < 4)%nat ->
+       code !! pa_add (u_pa (upt_entry vpn ie) va vpn) j = Some (nth_byte w j)) ->
+    _get_Mstatus_SXL ms_v = 'b"10" ->
+    is_aligned_vaddr (Virtaddr va) 4 = true ->
+    neq_vec (bits_of_virtaddr (Virtaddr va))
+       (sign_extend' 64 (subrange_vec_dec (bits_of_virtaddr (Virtaddr va)) (Z.sub 39 1) 0)) = false ->
+    autocast (T := mword) (subrange_vec_dec
+       (subrange_vec_dec (bits_of_virtaddr (Virtaddr va)) (Z.sub 39 1) 0) (Z.sub 39 1) pagesize_bits) = vpn ->
+    is_aligned_paddr (Physaddr (u_pa (upt_entry vpn ie) va vpn)) 4 = true ->
+    isRVC (subrange_vec_dec w 15 0) = false ->
+    (* decode: w is this RTYPE op *)
+    (forall s0, agree_on D_u s0 dstateU ->
+       exec (ext_decode w) s0 = Some (mk2 rs2 rs1 rd, s0)) ->
+    uint rd <> 0 ->
+    hw_config -∗
+    minstret_inv -∗
+    hart_state ↦ᵣ{ dq } HART_ACTIVE tt -∗
+    cur_privilege ↦ᵣ User -∗
+    mstatus ↦ᵣ ms_v -∗
+    scause ↦ᵣ sc_v -∗
+    stval ↦ᵣ stval_v -∗
+    sepc ↦ᵣ sepc_v -∗
+    tlb ↦ᵣ tlbvec -∗
+    pc_is va -∗
+    gpr_file g -∗
+    upt_inv root slots spec -∗
+    user_code -∗
+    user_data -∗
+    user_cfg -∗
+    ▷ (user_frame -∗ WP (Loop : expr riscv_lang) @ E {{ Φ }}) -∗
+    WP (Loop : expr riscv_lang) @ E {{ Φ }}.
+  Proof.
+    intros HN Hexec_op Hnlpad Hok Hvec Hchk0 HupdN Hpbmt0 Hcw HSXL Hval Hcanon
+           Hvpn_def Hpaal HnotRVC Hdec Hrd.
+    iIntros "#Hhw #Hinv Hhs Hpriv Hms Hsc Hstv Hsepc Htlbc [Hpcr Hnpc]
+             [%Hdom Hfmap] Hupt #Hcode Hdata Hcfg Hcont".
+    iApply (wp_instr_u_hit va vpn ie w (mk2 rs2 rs1 rd)
+              ms_v tlbvec E Φ HN Hvec Hchk0 HupdN Hpbmt0 Hcw HSXL Hval Hcanon
+              Hvpn_def Hpaal HnotRVC Hdec Hnlpad
+              with "Hhw Hinv Hhs Hpriv Hms Htlbc Hpcr Hcode Hcfg").
+    iIntros (σ Hpceq Hag Hpins) "[Hreg Hmem]".
+    assert (Hm1 : g !! Regidx rs1 = Some (g !!! Regidx rs1))
+      by (apply lookup_lookup_total_dom; apply Hdom).
+    assert (Hm2 : g !! Regidx rs2 = Some (g !!! Regidx rs2))
+      by (apply lookup_lookup_total_dom; apply Hdom).
+    assert (Hmd : g !! Regidx rd = Some (g !!! Regidx rd))
+      by (apply lookup_lookup_total_dom; apply Hdom).
+    iMod (reg_update _ nextPC _ (add_vec_int va 4) with "Hreg Hnpc") as "[Hreg Hnpc]".
+    iDestruct (big_sepM_lookup_acc _ _ _ _ Hm1 with "Hfmap") as "[Hr1c Hfb1]".
+    iDestruct (gpr_pt_value rs1 (g !!! Regidx rs1)
+                 (set_reg σ nextPC (add_vec_int va 4)) with "Hreg Hr1c") as %Hrv1.
+    iDestruct ("Hfb1" with "Hr1c") as "Hfmap".
+    iDestruct (big_sepM_lookup_acc _ _ _ _ Hm2 with "Hfmap") as "[Hr2c Hfb2]".
+    iDestruct (gpr_pt_value rs2 (g !!! Regidx rs2)
+                 (set_reg σ nextPC (add_vec_int va 4)) with "Hreg Hr2c") as %Hrv2.
+    iDestruct ("Hfb2" with "Hr2c") as "Hfmap".
+    iDestruct (big_sepM_insert_acc _ _ _ _ Hmd with "Hfmap") as "[Hrdc Hfins]".
+    rewrite (gpr_pt_nz rd _ Hrd).
+    iMod (reg_update _ (R_bitvector_64 (gpr_of_Z (uint rd))) _
+            (regval_into_reg (f (g !!! Regidx rs1) (g !!! Regidx rs2)))
+            with "Hreg Hrdc") as "[Hreg Hrdc]".
+    iDestruct ("Hfins" $! (regval_into_reg (f (g !!! Regidx rs1) (g !!! Regidx rs2)))
+                 with "[Hrdc]") as "Hfmap".
+    { rewrite (gpr_pt_nz rd _ Hrd). iExact "Hrdc". }
+    iModIntro.
+    iExists (set_reg (set_reg σ nextPC (add_vec_int va 4))
+               (R_bitvector_64 (gpr_of_Z (uint rd)))
+               (regval_into_reg (f (g !!! Regidx rs1) (g !!! Regidx rs2)))).
+    iSplitR.
+    { iPureIntro.
+      pose proof (Hexec_op rs2 rs1 rd (set_reg σ nextPC (add_vec_int va 4)) Hrd) as HE.
+      rewrite Hrv1 in HE. rewrite Hrv2 in HE.
+      exact HE. }
+    iSplitL "Hreg Hmem".
+    { unfold set_reg; cbn [sregs mem]. iFrame "Hreg Hmem". }
+    iIntros "Hhs' Hpriv' Hms' Htlbc' Hpc' Hcfg'".
+    assert (Lnpc : register_lookup nextPC
+             (set_reg (set_reg σ nextPC (add_vec_int va 4))
+                (R_bitvector_64 (gpr_of_Z (uint rd)))
+                (regval_into_reg (f (g !!! Regidx rs1) (g !!! Regidx rs2)))).(sregs)
+             = add_vec_int va 4).
+    { unfold set_reg; cbn [sregs].
+      tmig. rewrite register_lookup_set. reflexivity. }
+    iEval (rewrite Lnpc) in "Hpc'".
+    iNext.
+    iApply "Hcont".
+    rewrite /user_frame.
+    iExists ms_v, sc_v, stval_v, sepc_v, (add_vec_int va 4),
+            (<[Regidx rd := regval_into_reg (f (g !!! Regidx rs1) (g !!! Regidx rs2))]> g),
+            tlbvec.
+    iFrame "Hhs' Hpriv' Hms' Hsc Hstv Hsepc Htlbc' Hupt Hcode Hdata Hcfg'".
+    iSplitR; [iPureIntro; exact HSXL |].
+    iSplitR; [iPureIntro; exact Hok |].
+    iSplitL "Hpc' Hnpc"; [iFrame "Hpc' Hnpc" |].
+    iSplitR.
+    { iPureIntro. intro r. rewrite dom_insert_L. apply elem_of_union_r. apply Hdom. }
+    iExact "Hfmap".
+  Qed.
+
+  Lemma ustep_c_rtype2 (mk2 : mword 5 -> mword 5 -> mword 5 -> instruction) (f : mword 64 -> mword 64 -> mword 64)
+      (va : mword 64) (vpn : mword 27) (ie : uwalk_info) (h : mword 16) (ii : instruction)
+      (rs2 rs1 rd : mword 5)
+      (ms_v sc_v stval_v sepc_v : mword 64)
+      (g : gmap regidx (mword 64))
+      (tlbvec : vec (option TLB_Entry) (2 ^ 6))
+      E (Φ : mval -> iProp Σ) :
+    ↑minstretN ⊆ E ->
+    (* the op's register-generic execute fact (nonzero-rd form) *)
+    (forall (rs2' rs1' rd' : mword 5) s, uint rd' <> 0 ->
+       exec (execute (mk2 rs2' rs1' rd')) s
+       = Some (RETIRE_SUCCESS,
+               set_reg s (R_bitvector_64 (gpr_of_Z (uint rd')))
+                 (regval_into_reg
+                    (f (if Z.eqb (uint rs1') 0 then zero_reg
+                        else register_lookup
+                               (R_bitvector_64 (gpr_of_Z (uint rs1'))) s.(sregs))
+                       (if Z.eqb (uint rs2') 0 then zero_reg
+                        else register_lookup
+                               (R_bitvector_64 (gpr_of_Z (uint rs2'))) s.(sregs)))))) ->
+    upt_tlb_ok spec tlbvec ->
+    (* fetch-hit facts *)
+    vec_access_dec tlbvec (tlb_hash (__id 39) vpn) = Some (upt_entry vpn ie) ->
+    uw_check_ok (InstructionFetch tt) ie ->
+    update_PTE_Bits (uw_pte0 ie) (InstructionFetch tt) = None ->
+    _get_PTE_Ext_PBMT (ext_bits_of_PTE (uw_pte0 ie)) = ('b"00" : mword 2) ->
+    _get_Mstatus_SXL ms_v = 'b"10" ->
+    neq_vec (bits_of_virtaddr (Virtaddr va))
+       (sign_extend' 64 (subrange_vec_dec (bits_of_virtaddr (Virtaddr va)) (Z.sub 39 1) 0)) = false ->
+    autocast (T := mword) (subrange_vec_dec
+       (subrange_vec_dec (bits_of_virtaddr (Virtaddr va)) (Z.sub 39 1) 0) (Z.sub 39 1) pagesize_bits) = vpn ->
+    ((exists w4 : mword 32,
+        is_aligned_vaddr (Virtaddr va) 4 = true /\
+        is_aligned_paddr (Physaddr (u_pa (upt_entry vpn ie) va vpn)) 4 = true /\
+        (forall j : nat, (j < 4)%nat ->
+           code !! pa_add (u_pa (upt_entry vpn ie) va vpn) j = Some (nth_byte w4 j)) /\
+        h = subrange_vec_dec w4 15 0)
+     \/ (neq_vec (access_vec_dec va 0) ('b"0") = false /\
+         neq_vec (access_vec_dec va 1) ('b"0") = true /\
+         is_aligned_vaddr (Virtaddr va) 4 = false /\
+         is_aligned_paddr (Physaddr (u_pa (upt_entry vpn ie) va vpn)) 2 = true /\
+         (forall j : nat, (j < 2)%nat ->
+            code !! pa_add (u_pa (upt_entry vpn ie) va vpn) j = Some (nth_byte h j)))) ->
+    isRVC h = true ->
+    (* decode: h is a compressed RTYPE op expansion *)
+    (forall s0, agree_on D_u s0 dstateU ->
+       exec (ext_decode_compressed h) s0 = Some (ii, s0)) ->
+    (* the pure expansion to the base instruction *)
+    (forall s : mstate, exec (execute ii) s
+       = Some (ExecuteAs (mk2 rs2 rs1 rd), s)) ->
+    uint rd <> 0 ->
+    hw_config -∗
+    minstret_inv -∗
+    hart_state ↦ᵣ{ dq } HART_ACTIVE tt -∗
+    cur_privilege ↦ᵣ User -∗
+    mstatus ↦ᵣ ms_v -∗
+    scause ↦ᵣ sc_v -∗
+    stval ↦ᵣ stval_v -∗
+    sepc ↦ᵣ sepc_v -∗
+    tlb ↦ᵣ tlbvec -∗
+    pc_is va -∗
+    gpr_file g -∗
+    upt_inv root slots spec -∗
+    user_code -∗
+    user_data -∗
+    user_cfg -∗
+    ▷ (user_frame -∗ WP (Loop : expr riscv_lang) @ E {{ Φ }}) -∗
+    WP (Loop : expr riscv_lang) @ E {{ Φ }}.
+  Proof.
+    intros HN Hexec_op Hok Hvec Hchk0 HupdN Hpbmt0 HSXL Hcanon Hvpn_def
+           Hmode HisRVC Hdec Hexp Hrd.
+    iIntros "#Hhw #Hinv Hhs Hpriv Hms Hsc Hstv Hsepc Htlbc [Hpcr Hnpc]
+             [%Hdom Hfmap] Hupt #Hcode Hdata Hcfg Hcont".
+    iApply (wp_instr_c_hit va vpn ie h ii (mk2 rs2 rs1 rd)
+              ms_v tlbvec E Φ HN Hvec Hchk0 HupdN Hpbmt0 HSXL Hcanon
+              Hvpn_def Hmode HisRVC Hdec Hexp
+              with "Hhw Hinv Hhs Hpriv Hms Htlbc Hpcr Hcode Hcfg").
+    iIntros (σ Hpceq Hag Hpins) "[Hreg Hmem]".
+    assert (Hm1 : g !! Regidx rs1 = Some (g !!! Regidx rs1))
+      by (apply lookup_lookup_total_dom; apply Hdom).
+    assert (Hm2 : g !! Regidx rs2 = Some (g !!! Regidx rs2))
+      by (apply lookup_lookup_total_dom; apply Hdom).
+    assert (Hmd : g !! Regidx rd = Some (g !!! Regidx rd))
+      by (apply lookup_lookup_total_dom; apply Hdom).
+    iMod (reg_update _ nextPC _ (add_vec_int va 2) with "Hreg Hnpc") as "[Hreg Hnpc]".
+    iDestruct (big_sepM_lookup_acc _ _ _ _ Hm1 with "Hfmap") as "[Hr1c Hfb1]".
+    iDestruct (gpr_pt_value rs1 (g !!! Regidx rs1)
+                 (set_reg σ nextPC (add_vec_int va 2)) with "Hreg Hr1c") as %Hrv1.
+    iDestruct ("Hfb1" with "Hr1c") as "Hfmap".
+    iDestruct (big_sepM_lookup_acc _ _ _ _ Hm2 with "Hfmap") as "[Hr2c Hfb2]".
+    iDestruct (gpr_pt_value rs2 (g !!! Regidx rs2)
+                 (set_reg σ nextPC (add_vec_int va 2)) with "Hreg Hr2c") as %Hrv2.
+    iDestruct ("Hfb2" with "Hr2c") as "Hfmap".
+    iDestruct (big_sepM_insert_acc _ _ _ _ Hmd with "Hfmap") as "[Hrdc Hfins]".
+    rewrite (gpr_pt_nz rd _ Hrd).
+    iMod (reg_update _ (R_bitvector_64 (gpr_of_Z (uint rd))) _
+            (regval_into_reg (f (g !!! Regidx rs1) (g !!! Regidx rs2)))
+            with "Hreg Hrdc") as "[Hreg Hrdc]".
+    iDestruct ("Hfins" $! (regval_into_reg (f (g !!! Regidx rs1) (g !!! Regidx rs2)))
+                 with "[Hrdc]") as "Hfmap".
+    { rewrite (gpr_pt_nz rd _ Hrd). iExact "Hrdc". }
+    iModIntro.
+    iExists (set_reg (set_reg σ nextPC (add_vec_int va 2))
+               (R_bitvector_64 (gpr_of_Z (uint rd)))
+               (regval_into_reg (f (g !!! Regidx rs1) (g !!! Regidx rs2)))).
+    iSplitR.
+    { iPureIntro.
+      pose proof (Hexec_op rs2 rs1 rd (set_reg σ nextPC (add_vec_int va 2)) Hrd) as HE.
+      rewrite Hrv1 in HE. rewrite Hrv2 in HE.
+      exact HE. }
+    iSplitL "Hreg Hmem".
+    { unfold set_reg; cbn [sregs mem]. iFrame "Hreg Hmem". }
+    iIntros "Hhs' Hpriv' Hms' Htlbc' Hpc' Hcfg'".
+    assert (Lnpc : register_lookup nextPC
+             (set_reg (set_reg σ nextPC (add_vec_int va 2))
+                (R_bitvector_64 (gpr_of_Z (uint rd)))
+                (regval_into_reg (f (g !!! Regidx rs1) (g !!! Regidx rs2)))).(sregs)
+             = add_vec_int va 2).
+    { unfold set_reg; cbn [sregs].
+      tmig. rewrite register_lookup_set. reflexivity. }
+    iEval (rewrite Lnpc) in "Hpc'".
+    iNext.
+    iApply "Hcont".
+    rewrite /user_frame.
+    iExists ms_v, sc_v, stval_v, sepc_v, (add_vec_int va 2),
+            (<[Regidx rd := regval_into_reg (f (g !!! Regidx rs1) (g !!! Regidx rs2))]> g),
+            tlbvec.
+    iFrame "Hhs' Hpriv' Hms' Hsc Hstv Hsepc Htlbc' Hupt Hcode Hdata Hcfg'".
+    iSplitR; [iPureIntro; exact HSXL |].
+    iSplitR; [iPureIntro; exact Hok |].
+    iSplitL "Hpc' Hnpc"; [iFrame "Hpc' Hnpc" |].
+    iSplitR.
+    { iPureIntro. intro r. rewrite dom_insert_L. apply elem_of_union_r. apply Hdom. }
+    iExact "Hfmap".
+  Qed.
+
   (* ------------------------------------------------------------------ *)
   (* The DIRECT compressed single-source compute: the compressed          *)
   (* instruction runs its rX/wX chain itself (C_NOT, C_ZEXT_B) -- no      *)
@@ -7381,6 +7643,70 @@ Section WpUserExec.
                                   (R_bitvector_64 (gpr_of_Z (uint rs1'))) s.(sregs))
                           (if Z.eqb (uint rs2') 0 then zero_reg
                            else register_lookup
+                                  (R_bitvector_64 (gpr_of_Z (uint rs2'))) s.(sregs)))))))
+    \/
+    (* 33: fetch hit, GENERIC retiring two-source compute (MULW/DIV/REM/...) *)
+    (exists vpn i (w : mword 32) (mk2 : mword 5 -> mword 5 -> mword 5 -> instruction)
+            (f : mword 64 -> mword 64 -> mword 64)
+            (rs2 rs1 rd : mword 5),
+       vec_access_dec tlbvec (tlb_hash (__id 39) vpn) = Some (upt_entry vpn i) /\
+       uw_check_ok (InstructionFetch tt) i /\
+       update_PTE_Bits (uw_pte0 i) (InstructionFetch tt) = None /\
+       _get_PTE_Ext_PBMT (ext_bits_of_PTE (uw_pte0 i)) = ('b"00" : mword 2) /\
+       (forall j : nat, (j < 4)%nat ->
+          code !! pa_add (u_pa (upt_entry vpn i) va vpn) j = Some (nth_byte w j)) /\
+       is_aligned_vaddr (Virtaddr va) 4 = true /\
+       neq_vec (bits_of_virtaddr (Virtaddr va))
+         (sign_extend' 64 (subrange_vec_dec (bits_of_virtaddr (Virtaddr va)) (Z.sub 39 1) 0)) = false /\
+       autocast (T := mword) (subrange_vec_dec
+         (subrange_vec_dec (bits_of_virtaddr (Virtaddr va)) (Z.sub 39 1) 0) (Z.sub 39 1) pagesize_bits) = vpn /\
+       is_aligned_paddr (Physaddr (u_pa (upt_entry vpn i) va vpn)) 4 = true /\
+       isRVC (subrange_vec_dec w 15 0) = false /\
+       (forall s0, agree_on D_u s0 dstateU ->
+          exec (ext_decode w) s0 = Some (mk2 rs2 rs1 rd, s0)) /\
+       uint rd <> 0 /\
+       (forall (rs2' rs1' rd' : mword 5) s, uint rd' <> 0 ->
+          exec (execute (mk2 rs2' rs1' rd')) s
+          = Some (RETIRE_SUCCESS,
+                  set_reg s (R_bitvector_64 (gpr_of_Z (uint rd')))
+                    (regval_into_reg
+                       (f (if Z.eqb (uint rs1') 0 then zero_reg
+                           else register_lookup
+                                  (R_bitvector_64 (gpr_of_Z (uint rs1'))) s.(sregs))
+                          (if Z.eqb (uint rs2') 0 then zero_reg
+                           else register_lookup
+                                  (R_bitvector_64 (gpr_of_Z (uint rs2'))) s.(sregs)))))) /\
+       is_lpad_instruction (mk2 rs2 rs1 rd) = false)
+    \/
+    (* 34: RVC fetch hit, compressed expanding to a two-source compute *)
+    (exists vpn i (h : mword 16) (ii : instruction) (mk2 : mword 5 -> mword 5 -> mword 5 -> instruction)
+            (f : mword 64 -> mword 64 -> mword 64)
+            (rs2 rs1 rd : mword 5),
+       vec_access_dec tlbvec (tlb_hash (__id 39) vpn) = Some (upt_entry vpn i) /\
+       uw_check_ok (InstructionFetch tt) i /\
+       update_PTE_Bits (uw_pte0 i) (InstructionFetch tt) = None /\
+       _get_PTE_Ext_PBMT (ext_bits_of_PTE (uw_pte0 i)) = ('b"00" : mword 2) /\
+       neq_vec (bits_of_virtaddr (Virtaddr va))
+         (sign_extend' 64 (subrange_vec_dec (bits_of_virtaddr (Virtaddr va)) (Z.sub 39 1) 0)) = false /\
+       autocast (T := mword) (subrange_vec_dec
+         (subrange_vec_dec (bits_of_virtaddr (Virtaddr va)) (Z.sub 39 1) 0) (Z.sub 39 1) pagesize_bits) = vpn /\
+       c_fetch_mode va vpn i h /\
+       isRVC h = true /\
+       (forall s0, agree_on D_u s0 dstateU ->
+          exec (ext_decode_compressed h) s0 = Some (ii, s0)) /\
+       (forall s : mstate, exec (execute ii) s
+          = Some (ExecuteAs (mk2 rs2 rs1 rd), s)) /\
+       uint rd <> 0 /\
+       (forall (rs2' rs1' rd' : mword 5) s, uint rd' <> 0 ->
+          exec (execute (mk2 rs2' rs1' rd')) s
+          = Some (RETIRE_SUCCESS,
+                  set_reg s (R_bitvector_64 (gpr_of_Z (uint rd')))
+                    (regval_into_reg
+                       (f (if Z.eqb (uint rs1') 0 then zero_reg
+                           else register_lookup
+                                  (R_bitvector_64 (gpr_of_Z (uint rs1'))) s.(sregs))
+                          (if Z.eqb (uint rs2') 0 then zero_reg
+                           else register_lookup
                                   (R_bitvector_64 (gpr_of_Z (uint rs2'))) s.(sregs))))))).
 
   (* the assembled Löb step obligation, v1 coverage *)
@@ -7471,10 +7797,16 @@ Section WpUserExec.
                                                                 | [ (vpn & i & h & ii & op & f & rs2 & rs1 & rd & Hvec & Hchk &
                                                                      Hupd & Hpbmt & Hcanon & Hvpn_def & Hmode & HisRVC & Hdec &
                                                                      Hexp & Hrd & Hexec_op)
-                                                                  | (vpn & i & h & ii & mulop & f & rs2 & rs1 & rd & Hvec &
-                                                                     Hchk & Hupd & Hpbmt & Hcanon & Hvpn_def & Hmode & HisRVC &
-                                                                     Hdec & Hexp & Hrd & Hexec_op)
-                                                                  ] ] ] ] ] ] ] ] ] ] ] ] ] ] ] ]
+                                                                  | [ (vpn & i & h & ii & mulop & f & rs2 & rs1 & rd & Hvec &
+                                                                       Hchk & Hupd & Hpbmt & Hcanon & Hvpn_def & Hmode & HisRVC &
+                                                                       Hdec & Hexp & Hrd & Hexec_op)
+                                                                    | [ (vpn & i & w & mk2 & f & rs2 & rs1 & rd & Hvec & Hchk &
+                                                                         Hupd & Hpbmt & Hcw & Hval & Hcanon & Hvpn_def & Hpaal &
+                                                                         HnotRVC & Hdec & Hrd & Hexec_op & Hnlpad)
+                                                                      | (vpn & i & h & ii & mk2 & f & rs2 & rs1 & rd & Hvec &
+                                                                         Hchk & Hupd & Hpbmt & Hcanon & Hvpn_def & Hmode &
+                                                                         HisRVC & Hdec & Hexp & Hrd & Hexec_op)
+                                                                      ] ] ] ] ] ] ] ] ] ] ] ] ] ] ] ] ] ]
                                   ] ] ] ] ] ] ] ] ] ] ] ] ] ] ].
     - (* non-canonical *)
       iDestruct "Hk" as "[_ HkT]".
@@ -7693,6 +8025,20 @@ Section WpUserExec.
     - (* compressed -> retiring MUL *)
       iDestruct "Hk" as "[HkP _]".
       iApply (ustep_c_mul mulop f va vpn i h ii rs2 rs1 rd ms_v sc_v stval_v sepc_v g
+                tlbvec E Φ HN Hexec_op Hok Hvec Hchk Hupd Hpbmt HSXL
+                Hcanon Hvpn_def Hmode HisRVC Hdec Hexp Hrd
+                with "Hhw Hinv Hhs Hpriv Hms Hsc Hstv Hsepc Htlbc Hpc Hgpr Hupt
+                      Hcode Hdata Hcfg HkP").
+    - (* generic two-source compute (MULW/DIV/DIVW/REM/REMW/...) *)
+      iDestruct "Hk" as "[HkP _]".
+      iApply (ustep_rtype2 mk2 f va vpn i w rs2 rs1 rd ms_v sc_v stval_v sepc_v g
+                tlbvec E Φ HN Hexec_op Hnlpad Hok Hvec Hchk Hupd Hpbmt Hcw HSXL Hval
+                Hcanon Hvpn_def Hpaal HnotRVC Hdec Hrd
+                with "Hhw Hinv Hhs Hpriv Hms Hsc Hstv Hsepc Htlbc Hpc Hgpr Hupt
+                      Hcode Hdata Hcfg HkP").
+    - (* compressed -> generic two-source compute *)
+      iDestruct "Hk" as "[HkP _]".
+      iApply (ustep_c_rtype2 mk2 f va vpn i h ii rs2 rs1 rd ms_v sc_v stval_v sepc_v g
                 tlbvec E Φ HN Hexec_op Hok Hvec Hchk Hupd Hpbmt HSXL
                 Hcanon Hvpn_def Hmode HisRVC Hdec Hexp Hrd
                 with "Hhw Hinv Hhs Hpriv Hms Hsc Hstv Hsepc Htlbc Hpc Hgpr Hupt
